wip!

Tests/FBoundExample.lean
@@ -17,26 +17,26 @@ def group : FBound Nat Nat where
 @[reducible] def boolBound : Aux group (λ _value => Bool) where
   Member := λ _id => Bool
   lookup := λ _id => none
-  saveMember := λ bundle => bundle.snd
-  loadMetadata := λ id2 => id2.snd
+  saveMeta := λ bundle => bundle.snd
+  loadMeta := λ id2 => id2.snd
 
 /-- Second FBound instance: metadata is `Unit` per value. -/
 @[reducible] def unitBound : Aux group (λ _value => Unit) where
   Member := λ _id => Unit
   lookup := λ _id => none
-  saveMember := λ bundle => bundle.snd
-  loadMetadata := λ id2 => id2.snd
+  saveMeta := λ bundle => bundle.snd
+  loadMeta := λ id2 => id2.snd
 
 section roundtrip
 
 example :
-    boolBound.loadMetadata
-      ⟨group.save 42, boolBound.saveMember ⟨42, true⟩⟩ = true := by
+    boolBound.loadMeta
+      ⟨group.save 42, boolBound.saveMeta ⟨42, true⟩⟩ = true := by
   rfl
 
 example :
-    unitBound.loadMetadata
-      ⟨group.save 7, unitBound.saveMember ⟨7, ()⟩⟩ = () := by
+    unitBound.loadMeta
+      ⟨group.save 7, unitBound.saveMeta ⟨7, ()⟩⟩ = () := by
   rfl
 
 end roundtrip
@@ -46,8 +46,8 @@ section sharedGroup
 example :
     boolBound.Member (group.save 1) ×
       unitBound.Member (group.save 1) :=
-  ⟨boolBound.saveMember ⟨1, false⟩,
-    unitBound.saveMember ⟨1, ()⟩⟩
+  ⟨boolBound.saveMeta ⟨1, false⟩,
+    unitBound.saveMeta ⟨1, ()⟩⟩
 
 end sharedGroup
 
