Lp2lc/Active/STLC/__Infer_umbral.lean
@@ -50,7 +50,7 @@ def infer_prove [env: @ProvingEnv F] (trm : AST.Trm F) :
         Option (@ProvenCondition F env.base ⟨term, typ⟩) :=
       let id := env.base.trm2typCtx.save ⟨term, typ⟩
       (env.proofCtx.lookup id).map (λ member => by
-        simpa [id] using env.proofCtx.loadMetadata id member)
+        simpa [id] using env.proofCtx.loadMeta id member)
     match trm with
     | .val (.primitive repr) =>
       .yield ((proven (.val (.primitive repr)) .primitive).map
